wip

src/riot/asn1/ASN1.Spec.Value.IA5_STRING.fst
@@ -12,75 +12,42 @@ open FStar.Integers
 
 module B32 = FStar.Bytes
 
-let synth_asn1_ia5_string
-  (len: asn1_value_int32_of_type IA5_STRING)
-  (s32: parse_filter_refine (filter_asn1_ia5_string len))
-: GTot (value: datatype_of_asn1_type IA5_STRING{(dfst value) == len})
-= (|len, s32|)
-
-let lemma_synth_asn1_ia5_string_injective ()
-= ()
-
-noextract inline_for_extraction
-let synth_asn1_ia5_string_inverse
-  (len: asn1_value_int32_of_type IA5_STRING)
-  (value: datatype_of_asn1_type IA5_STRING{(dfst value) == len})
-: (s32: parse_filter_refine (filter_asn1_ia5_string len)
-             { value == synth_asn1_ia5_string len s32 })
+let synth_asn1_ia5_string_inverse len value
 = dsnd value
 
-// let parse_asn1_ia5_string
-// = parse_asn1_string
-//     (IA5_STRING)
-//     (dfst)
-//     (filter_asn1_ia5_string)
-//     (synth_asn1_ia5_string)
-//     (lemma_synth_asn1_ia5_string_injective ())
+let parse_asn1_ia5_string
+= parse_asn1_string
+    (IA5_STRING)
+    (dfst)
+    (filter_asn1_ia5_string)
+    (synth_asn1_ia5_string)
+    ()
 
-// let serialize_asn1_ia5_string
-// = serialize_asn1_string
-//     (IA5_STRING)
-//     (dfst)
-//     (filter_asn1_ia5_string)
-//     (synth_asn1_ia5_string)
-//     (synth_asn1_ia5_string_inverse)
-//     (lemma_synth_asn1_ia5_string_injective ())
-
-let lemma_serialize_asn1_ia5_string_unfold
-= lemma_serialize_asn1_string_unfold
+let serialize_asn1_ia5_string
+= serialize_asn1_string
     (IA5_STRING)
     (dfst)
     (filter_asn1_ia5_string)
     (synth_asn1_ia5_string)
     (synth_asn1_ia5_string_inverse)
-    (lemma_synth_asn1_ia5_string_injective ())
+    ()
 
-let lemma_serialize_asn1_ia5_string_size
-= lemma_serialize_asn1_string_size
+let parse_asn1_ia5_string_TLV
+= parse_asn1_string_TLV
+    (IA5_STRING)
+    (dfst)
+    (filter_asn1_ia5_string)
+    (synth_asn1_ia5_string)
+    ()
+
+let serialize_asn1_ia5_string_TLV
+= serialize_asn1_string_TLV
     (IA5_STRING)
     (dfst)
     (filter_asn1_ia5_string)
     (synth_asn1_ia5_string)
     (synth_asn1_ia5_string_inverse)
-    (lemma_synth_asn1_ia5_string_injective ())
-
-
-// let parse_asn1_ia5_string_TLV
-// = parse_asn1_string_TLV
-//     (IA5_STRING)
-//     (dfst)
-//     (filter_asn1_ia5_string)
-//     (synth_asn1_ia5_string)
-//     (lemma_synth_asn1_ia5_string_injective ())
-
-// let serialize_asn1_ia5_string_TLV
-// = serialize_asn1_string_TLV
-//     (IA5_STRING)
-//     (dfst)
-//     (filter_asn1_ia5_string)
-//     (synth_asn1_ia5_string)
-//     (synth_asn1_ia5_string_inverse)
-//     (lemma_synth_asn1_ia5_string_injective ())
+    ()
 
 let lemma_serialize_asn1_ia5_string_TLV_unfold x
 = lemma_serialize_asn1_string_TLV_unfold
@@ -89,7 +56,7 @@ let lemma_serialize_asn1_ia5_string_TLV_unfold x
     (filter_asn1_ia5_string)
     (synth_asn1_ia5_string)
     (synth_asn1_ia5_string_inverse)
-    (lemma_synth_asn1_ia5_string_injective ())
+    ()
     (x)
 
 let lemma_serialize_asn1_ia5_string_TLV_size x
@@ -99,11 +66,8 @@ let lemma_serialize_asn1_ia5_string_TLV_size x
     (filter_asn1_ia5_string)
     (synth_asn1_ia5_string)
     (synth_asn1_ia5_string_inverse)
-    (lemma_synth_asn1_ia5_string_injective ())
+    ()
     (x)
-
-let count_ia5_character x
-= dfst x
 
 let parse_asn1_ia5_string_TLV_with_character_bound lb ub
 = parse_asn1_string_TLV_with_character_bound
@@ -111,7 +75,7 @@ let parse_asn1_ia5_string_TLV_with_character_bound lb ub
     (dfst)
     (filter_asn1_ia5_string)
     (synth_asn1_ia5_string)
-    (lemma_synth_asn1_ia5_string_injective ())
+    ()
     (count_ia5_character)
     (lb)
     (ub)
@@ -123,7 +87,7 @@ let serialize_asn1_ia5_string_TLV_with_character_bound lb ub
     (filter_asn1_ia5_string)
     (synth_asn1_ia5_string)
     (synth_asn1_ia5_string_inverse)
-    (lemma_synth_asn1_ia5_string_injective ())
+    ()
     (count_ia5_character)
     (lb)
     (ub)
