src/riot/asn1/ASN1.Spec.Value.IA5_STRING.fsti
@@ -9,12 +9,6 @@ open FStar.Integers
 
 module B32 = FStar.Bytes
 
-(* ZT: Maybe we don't need to hide this module, which is
-       just instantiating another mudule. Since the lemmas'
-       types are also instantiating some meta predicates,
-       they are meanlingless unless a module friends this
-       module. *)
-
 let filter_asn1_ia5_string
   (len: asn1_value_int32_of_type IA5_STRING)
   (s32: B32.lbytes32 len)
@@ -22,100 +16,55 @@ let filter_asn1_ia5_string
 = let s = B32.reveal s32 in
   Seq.for_all valid_IA5_byte s
 
-val synth_asn1_ia5_string
+let synth_asn1_ia5_string
   (len: asn1_value_int32_of_type IA5_STRING)
   (s32: parse_filter_refine (filter_asn1_ia5_string len))
 : GTot (value: datatype_of_asn1_type IA5_STRING{(dfst value) == len})
-
-val lemma_synth_asn1_ia5_string_injective (_: unit)
-: Lemma (
-  forall (len: asn1_value_int32_of_type (IA5_STRING)).
-    synth_injective (synth_asn1_ia5_string len)
-)
+= (|len, s32|)
 
 noextract inline_for_extraction
 val synth_asn1_ia5_string_inverse
   (len: asn1_value_int32_of_type IA5_STRING)
   (value: datatype_of_asn1_type IA5_STRING{(dfst value) == len})
-: (s32: parse_filter_refine (filter_asn1_ia5_string len)
+: Tot (s32: parse_filter_refine (filter_asn1_ia5_string len)
              { value == synth_asn1_ia5_string len s32 })
 
-(* ZT: Exposing those two since the type of lemmas below
-       depends on their implementation *)
-let parse_asn1_ia5_string
-  (len: asn1_value_int32_of_type IA5_STRING)
-: parser (parse_asn1_string_kind IA5_STRING len)
-         (x: datatype_of_asn1_type IA5_STRING {dfst x == len})
-= parse_asn1_string
-    (IA5_STRING)
+val parse_asn1_ia5_string (len:asn1_value_int32_of_type IA5_STRING)
+: parser (parse_filter_kind (total_constant_size_parser_kind (v len)))
+    (x:datatype_of_asn1_type IA5_STRING{dfst x == len})
+
+val serialize_asn1_ia5_string (len:asn1_value_int32_of_type IA5_STRING)
+: serializer (parse_asn1_string IA5_STRING
     (dfst)
     (filter_asn1_ia5_string)
     (synth_asn1_ia5_string)
-    (lemma_synth_asn1_ia5_string_injective ())
-    (len)
+    () len)
 
-let serialize_asn1_ia5_string
-  (len: asn1_value_int32_of_type IA5_STRING)
-: serializer (parse_asn1_ia5_string len)
-= serialize_asn1_string
+let lemma_serialize_asn1_ia5_string_unfold
+= lemma_serialize_asn1_string_unfold
     (IA5_STRING)
     (dfst)
     (filter_asn1_ia5_string)
     (synth_asn1_ia5_string)
     (synth_asn1_ia5_string_inverse)
-    (lemma_synth_asn1_ia5_string_injective ())
-    (len)
+    ()
 
-val lemma_serialize_asn1_ia5_string_unfold
-  (len: asn1_value_int32_of_type IA5_STRING)
-  (x: datatype_of_asn1_type IA5_STRING { dfst x == len })
-: Lemma (
-  predicate_serialize_asn1_string_unfold
+let lemma_serialize_asn1_ia5_string_size
+= lemma_serialize_asn1_string_size
     (IA5_STRING)
     (dfst)
     (filter_asn1_ia5_string)
     (synth_asn1_ia5_string)
     (synth_asn1_ia5_string_inverse)
-    (lemma_synth_asn1_ia5_string_injective ())
-    (len)
-    (x)
-)
-
-val lemma_serialize_asn1_ia5_string_size
-  (len: asn1_value_int32_of_type IA5_STRING)
-  (x: datatype_of_asn1_type IA5_STRING { dfst x == len })
-: Lemma (
-  predicate_serialize_asn1_string_size
-    (IA5_STRING)
-    (dfst)
-    (filter_asn1_ia5_string)
-    (synth_asn1_ia5_string)
-    (synth_asn1_ia5_string_inverse)
-    (lemma_synth_asn1_ia5_string_injective ())
-    (len)
-    (x)
-)
+    ()
 
 let parse_asn1_ia5_string_TLV_kind = parse_asn1_string_TLV_kind IA5_STRING
 
-let parse_asn1_ia5_string_TLV
+val parse_asn1_ia5_string_TLV
 : parser parse_asn1_ia5_string_TLV_kind (datatype_of_asn1_type IA5_STRING)
-= parse_asn1_string_TLV
-    (IA5_STRING)
-    (dfst)
-    (filter_asn1_ia5_string)
-    (synth_asn1_ia5_string)
-    (lemma_synth_asn1_ia5_string_injective ())
 
-let serialize_asn1_ia5_string_TLV
+val serialize_asn1_ia5_string_TLV
 : serializer (parse_asn1_ia5_string_TLV)
-= serialize_asn1_string_TLV
-    (IA5_STRING)
-    (dfst)
-    (filter_asn1_ia5_string)
-    (synth_asn1_ia5_string)
-    (synth_asn1_ia5_string_inverse)
-    (lemma_synth_asn1_ia5_string_injective ())
 
 val lemma_serialize_asn1_ia5_string_TLV_unfold
   (x: datatype_of_asn1_type IA5_STRING)
@@ -126,7 +75,7 @@ val lemma_serialize_asn1_ia5_string_TLV_unfold
     (filter_asn1_ia5_string)
     (synth_asn1_ia5_string)
     (synth_asn1_ia5_string_inverse)
-    (lemma_synth_asn1_ia5_string_injective ())
+    ()
     (x)
 )
 
@@ -139,14 +88,14 @@ val lemma_serialize_asn1_ia5_string_TLV_size
     (filter_asn1_ia5_string)
     (synth_asn1_ia5_string)
     (synth_asn1_ia5_string_inverse)
-    (lemma_synth_asn1_ia5_string_injective ())
+    ()
     (x)
 )
 
-(* ZT: Consider to expose this if anything in `X509.BasicFields.RelativeDistinguishedName` got blocked. *)
-val count_ia5_character
+let count_ia5_character
   (x: datatype_of_asn1_type IA5_STRING)
-: (asn1_int32)
+: Tot (asn1_int32)
+= dfst x
 
 val parse_asn1_ia5_string_TLV_with_character_bound
   (lb: asn1_value_int32_of_type IA5_STRING)
@@ -157,4 +106,3 @@ val serialize_asn1_ia5_string_TLV_with_character_bound
   (lb: asn1_value_int32_of_type IA5_STRING)
   (ub: asn1_value_int32_of_type IA5_STRING { lb <= ub })
 : serializer (parse_asn1_ia5_string_TLV_with_character_bound lb ub)
-
